wip, elim/intro exists soundness

pulse/examples/dsls/mini_steel/Pulse.Elaborate.Pure.fst
@@ -47,22 +47,57 @@ let stt_ghost_tm = R.pack_ln (R.Tv_FVar stt_ghost_fv)
 let mk_stt_ghost_app (u:R.universe) (args:list R.term)
   : Tot R.term = 
   R.mk_app (R.pack_ln (R.Tv_UInst stt_ghost_fv [u])) (args_of args)
-
-let elim_exists_lid = mk_steel_wrapper_lid "elim_exists"
-let intro_exists_lid = mk_steel_wrapper_lid "intro_exists"
+let mk_stt_ghost_comp (u:R.universe) (a inames pre post:R.term) =
+  let t = R.pack_ln (R.Tv_UInst stt_ghost_fv [u]) in
+  let t = R.pack_ln (R.Tv_App t (a, R.Q_Explicit)) in
+  let t = R.pack_ln (R.Tv_App t (inames, R.Q_Explicit)) in
+  let t = R.pack_ln (R.Tv_App t (pre, R.Q_Explicit)) in
+  R.pack_ln (R.Tv_App t (post, R.Q_Explicit))
 
 let mk_total t = R.C_Total t
 let binder_of_t_q t q = RT.mk_binder (Sealed.seal "_") 0 t q
 let binder_of_t_q_s t q s = RT.mk_binder s 0 t q
 let bound_var i : R.term = R.pack_ln (R.Tv_BVar (R.pack_bv (RT.make_bv i tun)))
 let mk_name i : R.term = R.pack_ln (R.Tv_Var (R.pack_bv (RT.make_bv i tun))) 
+
 let arrow_dom = (R.term & R.aqualv)
-let mk_tot_arrow1 (f:arrow_dom) (out:R.term) : R.term =
+let mk_arrow (f:arrow_dom) (out:R.term) : R.term =
   let ty, q = f in
   R.pack_ln (R.Tv_Arrow (binder_of_t_q ty q) (R.pack_comp (mk_total out)))
-let mk_tot_arrow_with_name1 (s:Sealed.sealed string) (f:arrow_dom) (out:R.term) : R.term =
+let mk_arrow_with_name (s:Sealed.sealed string) (f:arrow_dom) (out:R.term) : R.term =
   let ty, q = f in
   R.pack_ln (R.Tv_Arrow (binder_of_t_q_s ty q s) (R.pack_comp (mk_total out)))
+let mk_abs ty qual t : R.term =  R.pack_ln (R.Tv_Abs (binder_of_t_q ty qual) t)
+let mk_abs_with_name s ty qual t : R.term =  R.pack_ln (R.Tv_Abs (binder_of_t_q_s ty qual s) t)
+
+
+let elim_exists_lid = mk_steel_wrapper_lid "elim_exists"
+let intro_exists_lid = mk_steel_wrapper_lid "intro_exists"
+
+let mk_exists (u:R.universe) (a p:R.term) =
+  let body = mk_abs a R.Q_Explicit p in
+  let t = R.pack_ln (R.Tv_UInst (R.pack_fv exists_lid) [u]) in
+  let t = R.pack_ln (R.Tv_App t (a, R.Q_Implicit)) in
+  R.pack_ln (R.Tv_App t (body, R.Q_Explicit))
+
+let mk_forall (u:R.universe) (a p:R.term) =
+  let body = mk_abs a R.Q_Explicit p in
+  let t = R.pack_ln (R.Tv_UInst (R.pack_fv forall_lid) [u]) in
+  let t = R.pack_ln (R.Tv_App t (a, R.Q_Implicit)) in
+  R.pack_ln (R.Tv_App t (body, R.Q_Explicit))
+
+let mk_elim_exists (u:R.universe) (a p:R.term) : R.term =
+  let t = R.pack_ln (R.Tv_UInst (R.pack_fv elim_exists_lid) [u]) in
+  let t = R.pack_ln (R.Tv_App t (a, R.Q_Implicit)) in
+  let p = mk_abs t R.Q_Explicit p in
+  R.pack_ln (R.Tv_App t (p, R.Q_Explicit))
+
+let mk_intro_exists (u:R.universe) (a p:R.term) (e:R.term) : R.term =
+  let t = R.pack_ln (R.Tv_UInst (R.pack_fv intro_exists_lid) [u]) in
+  let t = R.pack_ln (R.Tv_App t (a, R.Q_Implicit)) in
+  let p = mk_abs t R.Q_Explicit p in
+  let t = R.pack_ln (R.Tv_App t (p, R.Q_Explicit)) in
+  R.pack_ln (R.Tv_App t (e, R.Q_Explicit))
 
 let vprop_eq_tm t1 t2 =
   let open R in
@@ -75,9 +110,6 @@ let vprop_eq_tm t1 t2 =
   t
 
 let emp_inames_tm : R.term = R.pack_ln (R.Tv_FVar (R.pack_fv emp_inames_lid))
-
-let mk_abs ty qual t : R.term =  R.pack_ln (R.Tv_Abs (binder_of_t_q ty qual) t)
-let mk_abs_with_name s ty qual t : R.term =  R.pack_ln (R.Tv_Abs (binder_of_t_q_s ty qual s) t)
 
 let non_informative_witness_lid = mk_steel_wrapper_lid "non_informative_witness"
 let non_informative_witness_rt (u:R.universe) (a:R.term) : R.term =
@@ -158,7 +190,7 @@ let rec elab_term (top:term)
     | Tm_Arrow b q c ->
       let! ty = elab_term b.binder_ty in
       let! c = elab_comp c in
-      Some (mk_tot_arrow_with_name1 b.binder_ppname (ty, elab_qual q) c)
+      Some (mk_arrow_with_name b.binder_ppname (ty, elab_qual q) c)
 
     | Tm_Let t e1 e2 ->
       let! t = elab_term t in
@@ -188,18 +220,13 @@ let rec elab_term (top:term)
       Some (R.mk_app head [(l, Q_Explicit); (r, Q_Explicit)])
       
     | Tm_ExistsSL u t body
-    | Tm_ForallSL u t body ->    
+    | Tm_ForallSL u t body ->
+      let u = elab_universe u in
       let! t = elab_term t in
       let! b = elab_term body in
-      let body = R.pack_ln (R.Tv_Abs (binder_of_t_q t R.Q_Explicit) b) in
-      let head = 
-        let head_lid = 
-          if Tm_ExistsSL? top
-          then exists_lid
-          else forall_lid 
-        in
-        pack_ln (Tv_UInst (pack_fv head_lid) [elab_universe u]) in
-      Some (R.mk_app head ([(t, Q_Implicit); (body, Q_Explicit)]))
+      if Tm_ExistsSL? top
+      then Some (mk_exists u t b)
+      else Some (mk_forall u t b)
 
     | Tm_Inames ->
       Some (pack_ln (Tv_FVar (pack_fv inames_lid)))
@@ -388,4 +415,3 @@ and closing_pure_comp (x:pure_comp) (v:var) (i:index)
       closing_pure_term pre v i;
       closing_pure_term post v (i + 1)
 #pop-options
-
