pulse/examples/dsls/mini_steel/Pulse.Soundness.Exists.fsti
@@ -1,0 +1,18 @@
+module Pulse.Soundness.Exists
+
+open FStar.Reflection
+open Refl.Typing
+open Pulse.Elaborate.Pure
+
+val elim_exists_soundness
+  (#g:fstar_top_env)
+  (#u:universe)
+  (#a:term)
+  (#p:term)
+  (a_typing:typing g a (pack_ln (Tv_Type u)))
+  (p_typing:typing g (mk_abs a Q_Explicit p)
+                     (mk_arrow (a, Q_Explicit) vprop_tm))
+
+  : GTot (typing g (mk_elim_exists u a p) (mk_stt_ghost_comp u a emp_inames_tm
+                                             (mk_exists u a p)
+                                             (mk_abs a Q_Explicit p)))
